WIP: Advance proof of dm_bind and refactor the code

io/DM.IO.New.fst
@@ -11,8 +11,8 @@ open Free.IO.Call
 open Hist
 
 (** TODO:
-- [ ] define as io_sig, io_spec that is a struct { pre: ...; post: ...; }
-- [ ] define hist as Theo: hist a = hist_post a -> hist_pre a
+- [v] define as io_sig, io_spec that is a struct { pre: ...; post: ...; }
+- [v] define hist as Theo: hist a = hist_post a -> hist_pre a
 - [ ] prove bind
 - [ ] extract the 3 relevant files: the free monad, the hist monad, a sig file, and this one with the DM effect.
 - [ ] write a test file
@@ -30,54 +30,64 @@ The history is in reverse chronology order.
 At the end of an io computation, the trace will be
 (reverse of local trace) appended to the history. **)
 
-let rec is_open (fd:file_descr) (h: trace) :
-  Tot bool =
-  match h with
-  | [] -> false
-  | h :: tail -> match h with
-               | EOpenfile _ (Inl fd') ->
-                   if fd = fd' then true
-                   else is_open fd tail
-               | EClose fd' _ ->
-                    if fd = fd' then false
-                    else is_open fd tail
-               | _ -> is_open fd tail
-
-
-unfold
-let op_pre (cmd:io_cmds) (arg:io_args cmd) (h:trace) : Type0 =
-  match cmd with
-  | Openfile -> True
-  | Read -> is_open arg h
-  | Close -> is_open arg h
-
 (** Inspierd from Kenji's thesis (2.4.5) **)
-let rec io_theta #a
+let rec theta #a
   (m : io a) : hist a =
   match m with
-  | Return x -> hist_return a x
-  | Call cmd arg fnc ->
-    hist_bind
-      (res cmd)
-      a
-      (fun h p -> op_pre cmd arg h /\ (forall r. p r [convert_call_to_event cmd arg r]))
-      (fun r -> io_theta (fnc r))
+  | Return x -> hist_return x
+  | Call cmd arg k ->
+    hist_bind (io_wps cmd arg) (fun r -> theta (k r))
 
-unfold
-let stronger_wp #a (w1 w2 : hist a) : Type0 =
-  forall (post : hist_post a) (hist : trace). w1 hist post ==> w2 hist post
+let lemma_theta_is_monad_morphism_ret v h p :
+  Lemma
+    (theta (io_return v) == hist_return v) by (compute ()) = ()
 
+let lemma_theta_is_monad_morphism_bind (m:io 'a) (f:'a -> io 'b) :
+  Lemma
+    (theta (io_bind m f) == hist_bind (theta m) (fun x -> theta (f x))) = 
+  match m with
+  | Return x ->
+    calc (==) {
+      theta (io_bind (Return x) f);
+      == {} // unfold io_bind
+      theta (f x); 
+      == { _ by (tadmit ()) } // fold hist_bind
+      hist_bind (hist_return x) (fun x -> theta (f x));
+      == { _ by (compute ()) } // fold theta
+      hist_bind (theta (Return x)) (fun x -> theta (f x));
+    };
+    (** not sure why these asserts are needed: **)
+    assert (theta (io_bind m f) == hist_bind (theta m) (fun x -> theta (f x))) by (
+      rewrite_eqs_from_context ();
+      compute ();
+      assumption ()
+    )
+  | Call cmd arg k ->
+    calc (==) {
+      theta (io_bind (Call cmd arg k) f);
+      == { _ by (compute ()) } // unfold io_bind
+      theta (Call cmd arg (fun r -> io_bind (k r) f));
+      == { _ by (compute ()) } // unfold theta
+      hist_bind (io_wps cmd arg) (fun r -> theta (io_bind (k r) f));
+      == { _ by (tadmit ())} // apply this lemma again for (k r) and f
+      hist_bind (io_wps cmd arg) (fun r -> hist_bind (theta (k r)) (fun x -> theta (f x)));
+      == { _ by (tadmit ()) } // monad law 3
+      hist_bind (hist_bind (io_wps cmd arg) (fun r -> theta (k r))) (fun x -> theta (f x));
+      == { _ by (compute ()) } // fold theta
+      hist_bind (theta (Call cmd arg k)) (fun x -> theta (f x));
+    };
+    (** not sure why these asserts are needed: **)
+    assert (theta (io_bind (Call cmd arg k) f) == hist_bind (theta (Call cmd arg k)) (fun x -> theta (f x)))
+      by (assumption ());
+    assert (theta (io_bind m f) == hist_bind (theta m) (fun x -> theta (f x)))
+      by (rewrite_eqs_from_context (); assumption ())
+  
 // The Dijkstra Monad
 let dm (a:Type) (wp:hist a) =
-  (m:(io a){wp `stronger_wp` io_theta m})
+  (m:(io a){wp `hist_ord` theta m})
 
-let dm_return (a : Type) (x : a) : dm a (hist_return a x) =
-  io_return a x
-
-let lemma_dm_bind a b w wf (m : dm a w) (f : (x:a) -> dm b (wf x)) (post : hist_post b) (hist : trace) :
-  Lemma
-    (requires hist_bind _ _ w wf hist post)
-    (ensures io_theta (io_bind _ _ m f) hist post) = admit ()
+let dm_return (a : Type) (x : a) : dm a (hist_return x) =
+  io_return x
 
 let dm_bind
   (a b : Type)
@@ -85,9 +95,12 @@ let dm_bind
   (wp_f: a -> hist b)
   (v : dm a wp_v)
   (f : (x:a -> dm b (wp_f x))) :
-  Tot (dm b (hist_bind _ _ wp_v wp_f)) =
-  Classical.forall_intro_2 (Classical.move_requires_2 (lemma_dm_bind a b wp_v wp_f v f));
-  io_bind _ _ v f
+  Tot (dm b (hist_bind wp_v wp_f)) =
+  lemma_theta_is_monad_morphism_bind v f;
+  assert (wp_v `hist_ord` (theta v));
+  assert (forall r. (wp_f r) `hist_ord` (theta (f r)));
+  assume (hist_bind wp_v wp_f `hist_ord` hist_bind (theta v) (fun x -> theta (f x)));
+  io_bind v f
 
 let dm_subcomp (a:Type) (wp1 wp2: hist a) (f : dm a wp1) :
   Pure (dm a wp2)
@@ -95,12 +108,7 @@ let dm_subcomp (a:Type) (wp1 wp2: hist a) (f : dm a wp1) :
     (ensures fun _ -> True) =
   f
 
-let dm_if_then_else
-  (a : Type)
-  (wp1 wp2: hist a)
-  (f : dm a wp1)
-  (g : dm a wp2) (b : bool) :
-  Tot Type =
+let dm_if_then_else (a : Type) (wp1 wp2: hist a) (f : dm a wp1) (g : dm a wp2) (b : bool) : Type =
   dm a (hist_if_then_else wp1 wp2 b)
 
 total
@@ -118,23 +126,18 @@ layered_effect {
 }
 
 let elim_pure #a #w (f : unit -> PURE a w) :
-  Pure
-    a
+  Pure a
     (requires w (fun _ -> True))
-    (ensures fun r -> forall post. w post ==> post r)
-= FStar.Monotonic.Pure.elim_pure_wp_monotonicity_forall () ;
+    (ensures fun r -> forall post. w post ==> post r) =
+  FStar.Monotonic.Pure.elim_pure_wp_monotonicity_forall ();
   f ()
-
-unfold
-let hist_lift #a (w : pure_wp a) : hist a =
-  fun hist post -> w (fun x -> post x [])
 
 (** inspired from Alg **)
 let lift_pure_dm (a : Type) (w : pure_wp a) (f:(eqtype_as_type unit -> PURE a w)) :
-  Pure (dm a (hist_lift w)) (requires w (fun _ -> True)) (ensures fun _ -> True) =
+  Pure (dm a (wp_lift_pure_hist w)) (requires w (fun _ -> True)) (ensures fun _ -> True) =
   let r = elim_pure #a #w f in
-  let r' : dm a (hist_return _ r) = dm_return a r in
-  dm_subcomp _ (hist_return _ r) (hist_lift w) r'
+  let r' : dm a (hist_return r) = dm_return a r in
+  dm_subcomp _ (hist_return r) (wp_lift_pure_hist w) r'
 
 sub_effect PURE ~> IOwp = lift_pure_dm
 
@@ -142,17 +145,17 @@ effect IO
   (a:Type)
   (pre : trace -> Type0)
   (post : trace -> a -> trace -> Type0) =
-  IOwp a (fun (h:trace) (p:hist_post a) ->
+  IOwp a (fun (p:hist_post a) (h:trace) ->
     pre h /\ (forall res lt. post h res lt ==>  p res lt))
 
 let static_cmd
   (cmd : io_cmds)
   (argz : io_args cmd) :
   IO (io_resm cmd)
-    (requires (fun h -> op_pre cmd argz h))
+    (requires (fun h -> io_pres cmd argz h))
     (ensures (fun h r lt ->
         lt == [convert_call_to_event cmd argz r])) =
-  IOwp?.reflect(io_call cmd argz)
+  IOwp?.reflect (io_call cmd argz)
 
 let testStatic2 () : IO unit (fun _ -> True) (fun _ _ _ -> True) =
   let fd = static_cmd Openfile "../Makefile" in
