io/Hist.fst
@@ -2,49 +2,43 @@ module Hist
 
 open FStar.List.Tot.Base
 open Common
-open Free.IO
 
-// local_trace (from old to new)
-let hist_post a = a -> lt:trace -> Type0
+let trace = Free.IO.trace
 
-// past_events (from new to old; reversed compared with local_trace)
-let hist a = h:trace -> hist_post a -> Type0
+let hist_post a = r:a -> lt:trace -> Type0
+let hist_pre a = h:trace -> Type0
 
-unfold
-let hist_return (a:Type) (x:a) : hist a =
-  fun _ p -> p x []
+let hist a = hist_post a -> hist_pre a 
 
 unfold
-let compute_post
-  (a b:Type)
+let hist_return (x:'a) : hist 'a =
+  fun p _ -> p x []
+
+unfold 
+let hist_shift_post (p:hist_post 'a) (lt:trace) : hist_post 'a =
+  fun r lt' -> p r (lt @ lt')
+
+unfold
+let hist_post_bind
   (h:trace)
-  (kw : a -> hist b)
-  (p:hist_post b) :
-  Tot (hist_post a) =
-  (fun result local_trace ->
-      kw result
-       ((List.rev local_trace) @ h)
-       (fun result' local_trace' ->
-         p result' (local_trace @ local_trace')))
+  (kw : 'a -> hist 'b)
+  (p:hist_post 'b) :
+  Tot (hist_post 'a) =
+  fun r lt ->
+    kw r (hist_shift_post p lt) ((List.rev lt) @ h)
 
 unfold
-let hist_bind
-  (a:Type)
-  (b:Type)
-  (w : hist a)
-  (kw : a -> hist b) :
-  Tot (hist b) =
-  fun h p ->
-    w h (compute_post a b h kw p)
+let hist_bind (w : hist 'a) (kw : 'a -> hist 'b) : hist 'b =
+  fun p h -> w (hist_post_bind h kw p) h
 
-let gen_post #a (post:hist_post a) (cmd:io_cmds) arg res =
-  fun r local_trace ->
-    post r (convert_call_to_event cmd arg res :: local_trace)
+unfold
+let wp_lift_pure_hist (w : pure_wp 'a) : hist 'a =
+  fun p _ -> w (fun x -> p x [])
 
 unfold
 val hist_ord (#a : Type) : hist a -> hist a -> Type0
 let hist_ord wp1 wp2 = forall h p. wp1 h p ==> wp2 h p
 
 unfold
-let hist_if_then_else (#a:Type) (wp1 wp2:hist a) (b:bool) : hist a =
-  fun h p -> (b ==> wp1 h p) /\ ((~b) ==> wp2 h p)
+let hist_if_then_else (wp1 wp2:hist 'a) (b:bool) : hist 'a =
+  fun p h -> (b ==> wp1 p h) /\ ((~b) ==> wp2 p h)
